src/SDK/CMM/Defs.dfy
@@ -21,23 +21,17 @@ module {:extern "CMMDefs"} CMMDefs {
     method GetEncryptionMaterials(materialsRequest: Materials.EncryptionMaterialsRequest)
                                   returns (res: Result<Materials.ValidEncryptionMaterials>)
       requires Valid()
-      requires ValidAAD(materialsRequest.encryptionContext)
+      requires EncryptionContext.Serializable(materialsRequest.encryptionContext)
       requires materialsRequest.encryptionContext.Keys !! Materials.ReservedKeyValues
       ensures Valid()
       ensures res.Success? ==> res.value.plaintextDataKey.Some? && res.value.algorithmSuiteID.ValidPlaintextDataKey(res.value.plaintextDataKey.get)
       ensures res.Success? ==> |res.value.encryptedDataKeys| > 0
-      ensures res.Success? ==> ValidAAD(res.value.encryptionContext)
+      ensures res.Success? ==> EncryptionContext.Serializable(res.value.encryptionContext)
       ensures res.Success? ==>
         match res.value.algorithmSuiteID.SignatureType()
           case None => true
           case Some(sigType) =>
             res.value.signingKey.Some?
-
-    // The following predicate is a synonym for Encryption.Serializable and provides a workaround for a translation bug
-    // of "fuel" in trait-override checks in Dafny. https://github.com/dafny-lang/dafny/issues/422
-    static predicate ValidAAD(encryptionContext: EncryptionContext.Map) {
-      EncryptionContext.Serializable(encryptionContext)
-    }
 
     method DecryptMaterials(materialsRequest: Materials.ValidDecryptionMaterialsRequest)
                             returns (res: Result<Materials.ValidDecryptionMaterials>)
