test/SDK/Client.dfy
@@ -42,7 +42,7 @@ module {:extern "TestClient"} TestClient {
       var encryptionContext := map[keyA := valA];
       assert EncryptionContext.Serializable(encryptionContext) by {
         // To prove EncryptionContext.Serializable, we need to reveal the definition of that predicate:
-        reveal EncryptionContext.Serializable();
+        EncryptionContext.RevealSerializable(encryptionContext);
         // We also need to help the verifier with proving the KVPairsLength is small:
         calc {
           EncryptionContext.Length(encryptionContext);
